@prefix : <https://schema.org/> .
@prefix rdf: <http://www.w3.org/1999/02/22-rdf-syntax-ns#> .
@prefix rdfs: <http://www.w3.org/2000/01/rdf-schema#> .
@prefix xml: <http://www.w3.org/XML/1998/namespace> .


:usNPI a rdf:Property ;
    rdfs:label "usNPI" ;
    :domainIncludes :Physician ;
    :isPartOf <https://pending.schema.org> ;
    :rangeIncludes :Text ;
    :source <https://github.com/schemaorg/schemaorg/issues/3420> ;
    rdfs:comment  """An NationalPoviderIdentifier(NPI) is a unique identification number for covered health care providers, created to help send health information electronically more quickly and effectively.""";
    rdfs:subPropertyOf :identifier .

:IndividualPhysician a rdfs:Class ;
    rdfs:label "IndividualPhysician" ;
    rdfs:comment  """An individual medical practitioner. For their official address use [[address]], for affiliations to hospitals use [[hospitalAffiliation]]. 
The [[practicesAt]] property can be used to indicate [[MedicalOrganization]] hospitals, clinics, pharmacies etc. where this physician practices.""" ;
    rdfs:subClassOf :Physician .

:PhysiciansOffice a rdfs:Class ;
    rdfs:label "PhysiciansOffice" ;
    rdfs:comment  """A doctor's office or clinic.""" ;
    rdfs:subClassOf :Physician .

:practicesAt a rdf:Property ;
    rdfs:label "practicesAt" ;
    :domainIncludes :IndividualPhysician ;
    :isPartOf <https://pending.schema.org> ;
    :rangeIncludes :MedicalOrganization ;
    :source <https://github.com/schemaorg/schemaorg/issues/3420> ;
    rdfs:comment  """A [[MedicalOrganization]] where the [[IndividualPhysician]] practices.""" ;